Minor changes

ref_impl/src/verifier/experiments/fstar_experiments/project2/bosqueTerms.fst
@@ -107,7 +107,7 @@ let extractBool2 x = match x with
 (* ------------------------------------------------------------------------ *)
 
 (* Definition of equality relation on Bosque terms *)
-val eqTerm_aux : #n:nat 
+val eqTerm_aux : n:nat 
   -> (x:sequence bosqueTerm n) 
   -> sequence bosqueTerm n 
   -> Tot (z:bosqueTerm{isBool z \/ isError z}) (decreases x)
@@ -121,12 +121,12 @@ let rec eqTerm x y = match x, y with
 | BTypedString s1 ty1, BTypedString s2 ty2 -> BBool (s1 = s2 && eqType ty1 ty2)
 | BGUID s1 n1, BGUID s2 n2 -> BBool (s1 = s2 && n1 = n2)
 | BTuple n1 seq1, BTuple n2 seq2 -> if (n1 <> n2) then BError
-                                   else eqTerm_aux #n1 seq1 seq2
+                                   else eqTerm_aux n1 seq1 seq2
 // FIX: Include case for BRecord
 // | BError, BError -> BBool true
 | _, _ -> BError
 and 
-eqTerm_aux #n x y = match x with
+eqTerm_aux n x y = match x with
 | SNil -> (match y with
          | SNil -> BBool true
          | _ -> BError
@@ -134,7 +134,7 @@ eqTerm_aux #n x y = match x with
 | SCons x1 m xs1 -> (match y with
                  | SNil -> BError
                  | SCons y1 m' ys1 -> (match (eqTerm x1 y1) with
-                                  | BBool b1 -> (match (eqTerm_aux xs1 ys1) with
+                                  | BBool b1 -> (match (eqTerm_aux m xs1 ys1) with
                                                | BBool b2 -> BBool ((m = m') && b1 && b2)
                                                | _ -> BError
                                                )
@@ -143,22 +143,34 @@ eqTerm_aux #n x y = match x with
                  )
 
 (* Definition of greater than or equal relation on Bosque terms *)
-val greaterOrEq : bosqueTerm -> bosqueTerm -> Tot (x:bosqueTerm{isBool x \/ isError x})
+val greaterOrEq : x:bosqueTerm{isInt x} -> y:bosqueTerm{isInt x} -> Tot (x:bosqueTerm{isBool x \/ isError x})
 let greaterOrEq x y = match x, y with
 | BInt x1, BInt y1 -> BBool (x1 >= y1)
 // FIX: Include case for Strings
 | _, _ -> BError
 
+(* Tuple Type projector *)
+val nthTupleType : index:int -> dimension:nat -> x:bosqueTerm -> Tot (bosqueType)
+let rec nthTupleType index dimension y = match y with
+| BTuple 0 SNil -> if (index < 0 || dimension <> 0) then BErrorType else BNoneType
+| BTuple dimension'' (SCons x dimension' xs) -> 
+  if (index < 0 || dimension <> dimension'') then BErrorType else
+  if (index >= dimension) then BNoneType else
+  if index = 0 then getType x
+  else nthTupleType (index-1) dimension' (BTuple dimension' xs)
+| _ -> BErrorType
+
 (* Tuple projector *)
-assume val nthTuple : index:int -> dimension:nat -> x:bosqueTerm -> Tot (y:bosqueTerm{eqType (getType y) BIntType})
-// let rec nthTuple index dimension y = match y with
-// | BTuple 0 SNil -> if (index < 0 || dimension <> 0) then BError else BNone
-// | BTuple dimension'' (SCons x #dimension' xs) -> 
-//   if (index < 0 || dimension <> dimension'') then BError else
-//   if (index >= dimension) then BNone else
-//   if index = 0 then x
-//   else nthTuple (index-1) dimension' (BTuple dimension' xs)
-// | _ -> BError
+// val nthTuple : index:int -> dimension:nat -> x:bosqueTerm -> Tot (y:bosqueTerm{eqType (nthTupleType index dimension x) (getType y)})
+val nthTuple : index:int -> dimension:nat -> x:bosqueTerm -> Tot (y:bosqueTerm)
+let rec nthTuple index dimension y = match y with
+| BTuple 0 SNil -> if (index < 0 || dimension <> 0) then BError else BNone
+| BTuple dimension'' (SCons x' dimension' xs') -> 
+  if (index < 0 || dimension <> dimension'') then BError else
+  if (index >= dimension) then BNone else
+  if index = 0 then x'
+  else nthTuple (index-1) dimension' (BTuple dimension' xs')
+| _ -> BError
 
 // FIX: Implement the following function
 // (* Record projector *)
