ref_impl/src/verifier/experiments/fstar_experiments/project2/bosqueTypes.fst
@@ -155,71 +155,71 @@ lemma_eqTypeSeq_sym n x y = match x with
                   | SCons hd' m' tl' -> lemma_eqType_sym hd hd'; lemma_eqTypeSeq_sym m tl tl'
                   )
 
-val lemma_eqTypeSeq_trans : n:nat -> (x:sequence bosqueType n)
-  -> (y:sequence bosqueType n) 
-  -> (z:sequence bosqueType n)
-  -> Lemma (requires (eqTypeSeq n x y) && (eqTypeSeq n y z)) (ensures (eqTypeSeq n x z)) (decreases %[x; y; z])
-val lemma_eqType_trans : x:bosqueType
-  -> y:bosqueType 
-  -> z:bosqueType 
-  -> Lemma (requires (eqType x y) && (eqType y z)) (ensures (eqType x z)) (decreases %[x; y; z])
-let rec lemma_eqType_trans x y z = match x with
-| BAnyType -> ()
-| BSomeType -> ()
-| BTruthyType -> ()
-| BNoneType -> ()
-| BUnionType t1 t2 -> (match y with
-                     | BUnionType t1' t2' -> (match z with
-                                            | BUnionType t1'' t2'' -> lemma_eqType_trans t1 t1' t1''; 
-                                                                     lemma_eqType_trans t2 t2' t2'' 
-                                            | _ -> ()
-                                            )
-                     | _ -> ()
-                     )
-| BParseableType -> ()
-| BBoolType -> ()
-| BIntType -> ()
-| BFloatType -> ()
-| BRegexType -> ()
-| BTypedStringType t -> (match y with
-                       | BTypedStringType t' -> (match z with
-                                               | BTypedStringType t'' -> lemma_eqType_trans t t' t''
-                                               | _ -> ()
-                                               )
-                       | _ -> ()
-                       )
-| BGUIDType -> ()
-| BTupleType _ n seq -> (match y with
-                     | BTupleType _ n' seq' -> (match z with
-                                            | BTupleType _ n'' seq'' -> lemma_eqTypeSeq_trans n seq seq' seq''
-                                            | _ -> ()
-                                            )
-                     | _ -> ()
-                     )
-| BRecordType _ n seq -> ()
-| BFunctionType -> ()
-| BObjectType -> ()
-| BEnumType -> ()
-| BCustomKeyType -> ()
-| BKeyedType -> ()
-| BErrorType -> ()
-and 
-lemma_eqTypeSeq_trans n x y z = match x with
-| SNil -> (match y with 
-         | SNil -> ()
-         | SCons hd' m' tl' -> (match z with 
-                              | SNil -> ()
-                              | SCons hd'' m'' tl'' -> ()
-                              )
-         )
-| SCons hd m tl -> (match y with 
-                  | SNil -> ()
-                  | SCons hd' m' tl' -> (match z with 
-                                       | SNil -> ()
-                                       | SCons hd'' m'' tl'' -> lemma_eqType_trans hd hd' hd''; 
-                                                               lemma_eqTypeSeq_trans m tl tl' tl''
-                                       )
-                  )
+// val lemma_eqTypeSeq_trans : n:nat -> (x:sequence bosqueType n)
+//   -> (y:sequence bosqueType n) 
+//   -> (z:sequence bosqueType n)
+//   -> Lemma (requires (eqTypeSeq n x y) && (eqTypeSeq n y z)) (ensures (eqTypeSeq n x z)) (decreases %[x; y; z])
+// val lemma_eqType_trans : x:bosqueType
+//   -> y:bosqueType 
+//   -> z:bosqueType 
+//   -> Lemma (requires (eqType x y) && (eqType y z)) (ensures (eqType x z)) (decreases %[x; y; z])
+// let rec lemma_eqType_trans x y z = match x with
+// | BAnyType -> ()
+// | BSomeType -> ()
+// | BTruthyType -> ()
+// | BNoneType -> ()
+// | BUnionType t1 t2 -> (match y with
+//                      | BUnionType t1' t2' -> (match z with
+//                                             | BUnionType t1'' t2'' -> lemma_eqType_trans t1 t1' t1''; 
+//                                                                      lemma_eqType_trans t2 t2' t2'' 
+//                                             | _ -> ()
+//                                             )
+//                      | _ -> ()
+//                      )
+// | BParseableType -> ()
+// | BBoolType -> ()
+// | BIntType -> ()
+// | BFloatType -> ()
+// | BRegexType -> ()
+// | BTypedStringType t -> (match y with
+//                        | BTypedStringType t' -> (match z with
+//                                                | BTypedStringType t'' -> lemma_eqType_trans t t' t''
+//                                                | _ -> ()
+//                                                )
+//                        | _ -> ()
+//                        )
+// | BGUIDType -> ()
+// | BTupleType _ n seq -> (match y with
+//                      | BTupleType _ n' seq' -> (match z with
+//                                             | BTupleType _ n'' seq'' -> lemma_eqTypeSeq_trans n seq seq' seq''
+//                                             | _ -> ()
+//                                             )
+//                      | _ -> ()
+//                      )
+// | BRecordType _ n seq -> ()
+// | BFunctionType -> ()
+// | BObjectType -> ()
+// | BEnumType -> ()
+// | BCustomKeyType -> ()
+// | BKeyedType -> ()
+// | BErrorType -> ()
+// and 
+// lemma_eqTypeSeq_trans n x y z = match x with
+// | SNil -> (match y with 
+//          | SNil -> ()
+//          | SCons hd' m' tl' -> (match z with 
+//                               | SNil -> ()
+//                               | SCons hd'' m'' tl'' -> ()
+//                               )
+//          )
+// | SCons hd m tl -> (match y with 
+//                   | SNil -> ()
+//                   | SCons hd' m' tl' -> (match z with 
+//                                        | SNil -> ()
+//                                        | SCons hd'' m'' tl'' -> lemma_eqType_trans hd hd' hd''; 
+//                                                                lemma_eqTypeSeq_trans m tl tl' tl''
+//                                        )
+//                   )
 
 (* Definition to encode the subtype relation on Bosque types 
    i.e. forall x y . subtypeOf x y <===> x :> y *)
